CallFFI of lab-to-target now cheat-free

compiler1/semantics/labPropsScript.sml
@@ -82,4 +82,102 @@ val write_bytearray_const = store_thm("write_bytearray_const[simp]",
   \\ rpt strip_tac \\ BasicProvers.EVERY_CASE_TAC
   \\ fs [labSemTheory.upd_mem_def]);
 
+val good_dimindex_def = Define `
+  good_dimindex (:'a) <=> dimindex (:'a) = 32 \/ dimindex (:'a) = 64`;
+
+val get_byte_set_byte = store_thm("get_byte_set_byte",
+  ``good_dimindex (:'a) ==>
+    (get_byte a (set_byte (a:'a word) b w be) be = b)``,
+  fs [get_byte_def,set_byte_def,LET_DEF]
+  \\ fs [fcpTheory.CART_EQ,w2w,good_dimindex_def] \\ rpt strip_tac
+  \\ `i < dimindex (:'a)` by decide_tac
+  \\ fs [word_or_def,fcpTheory.FCP_BETA,word_lsr_def,word_lsl_def]
+  \\ `i + byte_index a be < dimindex (:'a)` by
+   (fs [byte_index_def,LET_DEF] \\ rw []
+    \\ `w2n a MOD 4 < 4` by (match_mp_tac MOD_LESS \\ decide_tac)
+    \\ `w2n a MOD 8 < 8` by (match_mp_tac MOD_LESS \\ decide_tac)
+    \\ decide_tac)
+  \\ fs [word_or_def,fcpTheory.FCP_BETA,word_lsr_def,word_lsl_def,
+         word_slice_alt_def,w2w] \\ rfs []
+  \\ `~(i + byte_index a be < byte_index a be)` by decide_tac
+  \\ `~(byte_index a be + 8 <= i + byte_index a be)` by decide_tac
+  \\ fs [])
+
+val byte_index_LESS_IMP = prove(
+  ``(dimindex (:'a) = 32 \/ dimindex (:'a) = 64) /\
+    byte_index (a:'a word) be < byte_index (a':'a word) be /\ i < 8 ==>
+    byte_index a be + i < byte_index a' be /\
+    byte_index a be <= i + byte_index a' be /\
+    byte_index a be + 8 <= i + byte_index a' be /\
+    i + byte_index a' be < byte_index a be + dimindex (:α)``,
+  fs [byte_index_def,LET_DEF] \\ Cases_on `be` \\ fs []
+  \\ rpt strip_tac \\ rfs [] \\ fs []
+  \\ `w2n a MOD 4 < 4` by (match_mp_tac MOD_LESS \\ decide_tac)
+  \\ `w2n a' MOD 4 < 4` by (match_mp_tac MOD_LESS \\ decide_tac)
+  \\ `w2n a MOD 8 < 8` by (match_mp_tac MOD_LESS \\ decide_tac)
+  \\ `w2n a' MOD 8 < 8` by (match_mp_tac MOD_LESS \\ decide_tac)
+  \\ decide_tac);
+
+val NOT_w2w_bit = prove(
+  ``8 <= i /\ i < dimindex (:'b) ==> ~((w2w:word8->'b word) w ' i)``,
+  rpt strip_tac \\ rfs [w2w] \\ decide_tac);
+
+val LESS4 = DECIDE ``n < 4 <=> (n = 0) \/ (n = 1) \/ (n = 2) \/ (n = 3:num)``
+val LESS8 = DECIDE ``n < 8 <=> (n = 0) \/ (n = 1) \/ (n = 2) \/ (n = 3:num) \/
+                               (n = 4) \/ (n = 5) \/ (n = 6) \/ (n = 7)``
+
+val DIV_EQ_DIV_IMP = prove(
+  ``0 < d /\ n <> n' /\ (n DIV d * d = n' DIV d * d) ==> n MOD d <> n' MOD d``,
+  rpt strip_tac \\ Q.PAT_ASSUM `n <> n'` mp_tac \\ fs []
+  \\ MP_TAC (Q.SPEC `d` DIVISION) \\ fs []
+  \\ rpt strip_tac \\ pop_assum (fn th => once_rewrite_tac [th])
+  \\ fs []);
+
+val get_byte_set_byte_diff = store_thm("get_byte_set_byte_diff",
+  ``good_dimindex (:'a) /\ a <> a' /\ (byte_align a = byte_align a') ==>
+    (get_byte a (set_byte (a':'a word) b w be) be = get_byte a w be)``,
+  fs [get_byte_def,set_byte_def,LET_DEF] \\ rpt strip_tac
+  \\ `byte_index a be <> byte_index a' be` by
+   (fs [good_dimindex_def]
+    THENL
+     [`w2n a MOD 4 < 4 /\ w2n a' MOD 4 < 4` by fs []
+      \\ `w2n a MOD 4 <> w2n a' MOD 4` by
+       (fs [alignmentTheory.byte_align_def,byte_index_def] \\ rfs [LET_DEF]
+        \\ Cases_on `a` \\ Cases_on `a'` \\ fs [w2n_n2w] \\ rw []
+        \\ rfs [alignmentTheory.align_w2n]
+        \\ `(n DIV 4 * 4 + n MOD 4) < dimword (:'a) /\
+            (n' DIV 4 * 4 + n' MOD 4) < dimword (:'a)` by
+          (METIS_TAC [DIVISION,DECIDE ``0<4:num``])
+        \\ `(n DIV 4 * 4) < dimword (:'a) /\
+            (n' DIV 4 * 4) < dimword (:'a)` by decide_tac
+        \\ match_mp_tac DIV_EQ_DIV_IMP \\ fs []),
+      `w2n a MOD 8 < 8 /\ w2n a' MOD 8 < 8` by fs []
+      \\ `w2n a MOD 8 <> w2n a' MOD 8` by
+       (fs [alignmentTheory.byte_align_def,byte_index_def] \\ rfs [LET_DEF]
+        \\ Cases_on `a` \\ Cases_on `a'` \\ fs [w2n_n2w] \\ rw []
+        \\ rfs [alignmentTheory.align_w2n]
+        \\ `(n DIV 8 * 8 + n MOD 8) < dimword (:'a) /\
+            (n' DIV 8 * 8 + n' MOD 8) < dimword (:'a)` by
+          (METIS_TAC [DIVISION,DECIDE ``0<8:num``])
+        \\ `(n DIV 8 * 8) < dimword (:'a) /\
+            (n' DIV 8 * 8) < dimword (:'a)` by decide_tac
+        \\ match_mp_tac DIV_EQ_DIV_IMP \\ fs [])]
+    \\ full_simp_tac bool_ss [LESS4,LESS8] \\ fs [] \\ rfs []
+    \\ fs [byte_index_def,LET_DEF] \\ rw [])
+  \\ fs [fcpTheory.CART_EQ,w2w,good_dimindex_def] \\ rpt strip_tac
+  \\ `i' < dimindex (:'a)` by decide_tac
+  \\ fs [word_or_def,fcpTheory.FCP_BETA,word_lsr_def,word_lsl_def]
+  \\ `i' + byte_index a be < dimindex (:'a)` by
+   (fs [byte_index_def,LET_DEF] \\ rw []
+    \\ `w2n a MOD 4 < 4` by (match_mp_tac MOD_LESS \\ decide_tac)
+    \\ `w2n a MOD 8 < 8` by (match_mp_tac MOD_LESS \\ decide_tac)
+    \\ decide_tac)
+  \\ fs [word_or_def,fcpTheory.FCP_BETA,word_lsr_def,word_lsl_def,
+         word_slice_alt_def,w2w] \\ rfs []
+  \\ fs [DECIDE ``m <> n <=> m < n \/ n < m:num``]
+  \\ Cases_on `w ' (i' + byte_index a be)` \\ fs []
+  \\ imp_res_tac byte_index_LESS_IMP
+  \\ fs [w2w] \\ TRY (match_mp_tac NOT_w2w_bit)
+  \\ fs [] \\ decide_tac)
+
 val _ = export_theory();
